code/ecdsa/Hacl.Impl.EC.Masking.ScalarAccess.fst
@@ -26,6 +26,7 @@ open Hacl.Impl.EC.Masking.ScalarAccess.Lemmas
 
 #set-options "--fuel 0 --ifuel 0 --z3rlimit 200"
 
+inline_for_extraction
 val getScalarBit_leftEndian: #c: curve 
   -> #buf_type: buftype 
   -> s:lbuffer_t buf_type uint8 (getScalarLenBytes c) 
@@ -41,7 +42,7 @@ let getScalarBit_leftEndian #c #buf_type s n =
   to_u64 ((s.(getScalarLenBytes c -. 1ul -. n /. 8ul) >>. (n %. 8ul)) &. u8 1)
 
 
-inline_for_extraction noextract
+inline_for_extraction
 val getScalarBit_l: #c: curve 
   -> #buf_type: buftype 
   -> s:lbuffer_t buf_type uint8 (getScalarLenBytes c) 
@@ -69,7 +70,7 @@ let getScalarBit_l #c #b s n =
   pop_frame();
   result
 
-
+inline_for_extraction
 val getScalar_4: #c: curve
   -> #buf_type: buftype 
   -> s: scalar_t #buf_type #c
@@ -90,36 +91,28 @@ let getScalar_4 #c scalar i =
   let bitShift = logand i (size 1) in 
     logand_mask i (size 1) 1; 
   let bitShiftAsPrivate = size_to_uint32 bitShift in 
-  
-  let mask = cmovznz01 (u32 0xf0) (u32 0x0f) bitShiftAsPrivate in  
-  let shiftMask = cmovznz01 (size 0x4) (size 0x0) bitShift in
-  
-  let result0 = logand word mask in 
-  let result = shift_right result0 shiftMask in 
 
-  let index = v i in 
-
-  if index % 2 = 0 then 
+  let leftWord = shift_right word (size 0x4) in 
+  let rightWord = logand word (u32 0x0f) in 
+  
+  let result = cmovznz01 leftWord rightWord bitShiftAsPrivate in 
+ 
+  if v i % 2 = 0 then 
     begin
-      logand_spec word mask;
-      lemma_and_both_parts_32 word mask;
-      UInt.logand_lemma_1 #4 (v (get_low_part_4 word));
-      UInt.logand_mask #32 (v word / pow2 4) 4; 
-      assert (v result ==  (v (Lib.Sequence.index (as_seq h0 scalar) (index / 2)) / pow2 4) % pow2 4);
-
+      assert (v result ==  (v (Lib.Sequence.index (as_seq h0 scalar) (v i / 2)) / pow2 4) % pow2 4);
       let s = as_seq h0 scalar in 
       calc (==) {
 	v result;
-	   (==) {lemma_index_scalar_as_nat #c s (index / 2)}
-	((scalar_as_nat #c s / pow2 (v (getScalarLen c) - (index + 2) * 4) % pow2 8) / pow2 4) % pow2 4; 
-	  (==) {pow2_modulo_division_lemma_1 (scalar_as_nat #c s / pow2 (v (getScalarLen c) - (index + 2) * 4)) 4 8}
-	((scalar_as_nat #c s / pow2 (v (getScalarLen c) - (index + 2) * 4) / pow2 4) % pow2 4) % pow2 4;
-	  (==) {lemma_mod_twice ((scalar_as_nat #c s / pow2 (v (getScalarLen c) - (index + 2) * 4) / pow2 4)) (pow2 4)}
-	(scalar_as_nat #c s / pow2 (v (getScalarLen c) - (index + 2) * 4) / pow2 4) % pow2 4; };
-
+	   (==) {lemma_index_scalar_as_nat #c s (v i / 2)}
+	((scalar_as_nat #c s / pow2 (v (getScalarLen c) - (v i  + 2) * 4) % pow2 8) / pow2 4) % pow2 4; 
+	  (==) {pow2_modulo_division_lemma_1 (scalar_as_nat #c s / pow2 (v (getScalarLen c) - (v i  + 2) * 4)) 4 8}
+	((scalar_as_nat #c s / pow2 (v (getScalarLen c) - (v i  + 2) * 4) / pow2 4) % pow2 4) % pow2 4;
+	  (==) {lemma_mod_twice ((scalar_as_nat #c s / pow2 (v (getScalarLen c) - (v i + 2) * 4) / pow2 4)) (pow2 4)}
+	(scalar_as_nat #c s / pow2 (v (getScalarLen c) - (v i + 2) * 4) / pow2 4) % pow2 4; };
+	
       calc (==) {
-	(scalar_as_nat #c s / pow2 (v (getScalarLen c) - (index + 2) * 4) / pow2 4);
-	(==) {division_multiplication_lemma (scalar_as_nat #c s) (pow2 (v (getScalarLen c) - (index + 2) * 4)) (pow2 4)}
+	(scalar_as_nat #c s / pow2 (v (getScalarLen c) - (v i + 2) * 4) / pow2 4);
+	(==) {division_multiplication_lemma (scalar_as_nat #c s) (pow2 (v (getScalarLen c) - (v i  + 2) * 4)) (pow2 4)}
 	scalar_as_nat #c s / (pow2 (v (getScalarLen c) - (v i + 2) * 4) * pow2 4);
 	(==) {pow2_plus (v (getScalarLen c) - (v i + 2) * 4) 4} 
 	scalar_as_nat #c s / (pow2 (v (getScalarLen c) - (v i + 1) * 4));}
@@ -127,28 +120,25 @@ let getScalar_4 #c scalar i =
       end
   else
     begin
-
-      logand_mask word mask 4;
-      assert(v result = v (Lib.Sequence.index (as_seq h0 scalar) (index / 2)) % pow2 4);
-      
+      logand_mask word (u32 0x0f) 4;
+      assert(v result = v (Lib.Sequence.index (as_seq h0 scalar) (v i  / 2)) % pow2 4);
       let s = as_seq h0 scalar in 
 
       calc (==) {
 	v result;
       (==) {}
-	v (Lib.Sequence.index (as_seq h0 scalar) (index / 2)) % pow2 4;
-      (==) {lemma_index_scalar_as_nat #c s (index / 2)}
-	(scalar_as_nat #c s / pow2 (v (getScalarLen c) - (index / 2 + 1) * 8) % pow2 8) % pow2 4;
-      (==) {euclidean_division_definition index 2}
-	(scalar_as_nat #c s / pow2 (v (getScalarLen c) - (index + 1) * 4) % pow2 8) % pow2 4;
-      (==) {pow2_modulo_modulo_lemma_1 (scalar_as_nat #c s / pow2 (v (getScalarLen c) - (index + 1) * 4)) 4 8}
-      	scalar_as_nat #c s / pow2 (v (getScalarLen c) - (index + 1) * 4) % pow2 4; }
+	v (Lib.Sequence.index (as_seq h0 scalar) (v i  / 2)) % pow2 4;
+      (==) {lemma_index_scalar_as_nat #c s (v i  / 2)}
+	(scalar_as_nat #c s / pow2 (v (getScalarLen c) - (v i  / 2 + 1) * 8) % pow2 8) % pow2 4;
+      (==) {euclidean_division_definition (v i)  2}
+	(scalar_as_nat #c s / pow2 (v (getScalarLen c) - (v i  + 1) * 4) % pow2 8) % pow2 4;
+      (==) {pow2_modulo_modulo_lemma_1 (scalar_as_nat #c s / pow2 (v (getScalarLen c) - (v i + 1) * 4)) 4 8}
+      	scalar_as_nat #c s / pow2 (v (getScalarLen c) - (v i + 1) * 4) % pow2 4; }
     end;
-
+  
   result
 
-
-inline_for_extraction noextract
+inline_for_extraction
 val getScalar_4_byBit: #c: curve
   -> #buf_type: buftype 
   -> s: scalar_t #buf_type #c
@@ -170,52 +160,45 @@ let getScalar_4_byBit #c s i =
   let bit3 = shift_left (getScalarBit_leftEndian s (bit -! 3ul)) 0ul in 
 
   let r = logxor (logxor bit0 bit1) (logxor bit2 bit3) in 
-
-
-  let l = v (getScalarLen c) in 
   
-  assert(v bit0 = v (ith_bit (as_seq h0 s) (l - 1 - 4 * v i)) * 8);
-  assert(v bit1 = v (ith_bit (as_seq h0 s) (l - 1 - 4 * v i - 1)) * 4);
-  assert(v bit2 = v (ith_bit (as_seq h0 s) (l - 1 - 4 * v i - 2)) * 2);
-  assert(v bit3 = v (ith_bit (as_seq h0 s) (l - 1 - 4 * v i - 3)));
+  assert(v bit0 = v (ith_bit (as_seq h0 s) (v (getScalarLen c) - 1 - 4 * v i)) * 8);
+  assert(v bit1 = v (ith_bit (as_seq h0 s) (v (getScalarLen c) - 1 - 4 * v i - 1)) * 4);
+  assert(v bit2 = v (ith_bit (as_seq h0 s) (v (getScalarLen c) - 1 - 4 * v i - 2)) * 2);
+  assert(v bit3 = v (ith_bit (as_seq h0 s) (v (getScalarLen c) - 1 - 4 * v i - 3)));
 
   logxor_spec bit0 bit1;
   logxor_spec bit2 bit3;
   logxor_spec (logxor bit0 bit1) (logxor bit2 bit3);
   lemma_xor_of_4 
-    (ith_bit (as_seq h0 s) (l - 1 - 4 * v i))
-    (ith_bit (as_seq h0 s) (l - 1 - 4 * v i - 1)) 
-    (ith_bit (as_seq h0 s) (l - 1 - 4 * v i - 2))
-    (ith_bit (as_seq h0 s) (l - 1 - 4 * v i - 3));
+    (ith_bit (as_seq h0 s) (v (getScalarLen c) - 1 - 4 * v i))
+    (ith_bit (as_seq h0 s) (v (getScalarLen c) - 1 - 4 * v i - 1)) 
+    (ith_bit (as_seq h0 s) (v (getScalarLen c) - 1 - 4 * v i - 2))
+    (ith_bit (as_seq h0 s) (v (getScalarLen c) - 1 - 4 * v i - 3)); 
 
   scalar_as_nat_def #c (as_seq h0 s) (4 * v i + 1);
   scalar_as_nat_def #c (as_seq h0 s) (4 * v i + 2);
   scalar_as_nat_def #c (as_seq h0 s) (4 * v i + 3);
   scalar_as_nat_def #c (as_seq h0 s) (4 * v i + 4);
 
-  scalar_as_sub_radix4 (as_seq h0 s) (v i); 
+  scalar_as_sub_radix4 (as_seq h0 s) (v i);
 
   r
 
 
-
-
 open Hacl.Impl.EC.Precomputed
+
 
 inline_for_extraction noextract
 val getPointPrecomputedMixed_: #c: curve -> scalar: scalar_t #MUT #c -> 
-  i:size_t{v i < 64} -> pointToAdd: lbuffer uint64 (size 8) ->
+  i:size_t{v i < 64} -> pointToAdd: pointAffine c ->
   Stack unit 
   (requires fun h -> live h scalar /\ live h pointToAdd)
   (ensures fun h0 _ h1 -> True)
 
 let getPointPrecomputedMixed_ #c scalar i pointToAdd = 
-  push_frame();
-    let bits = getScalar_4_byBit scalar i in 
-  (*   let r =  shift_right (to_u64 bits) 18ul in 
-    let bits = getScalar_4 #c scalar i in *)
-   let invK h (k: nat) = True in 
-    Lib.Loops.for 0ul 16ul invK
+  let bits = getScalar_4 scalar i in 
+  let invK h (k: nat) = True in 
+  Lib.Loops.for 0ul 16ul invK
     (fun k -> 
       recall_contents points_radix_16 (Lib.Sequence.of_list points_radix_16_list_p256);
       let mask = eq_mask (to_u64 bits) (to_u64 k) in 
@@ -224,8 +207,7 @@ let getPointPrecomputedMixed_ #c scalar i pointToAdd =
 
       admit();
       copy_conditional #c (sub pointToAdd (size 0) (size 4)) lut_cmb_x mask;
-      copy_conditional #c (sub pointToAdd (size 4) (size 4)) lut_cmb_y mask);
-  pop_frame()
+      copy_conditional #c (sub pointToAdd (size 4) (size 4)) lut_cmb_y mask)
 
 
 let getPointPrecomputedMixed_p256 = getPointPrecomputedMixed_ #P256
