specs/ecdsa/Spec.ECC.fst
@@ -546,11 +546,9 @@ let rec scalar_as_nat_ #c s i =
 
 #push-options "--fuel 1 --ifuel 1 --z3rlimit 100"
 
-val scalar_as_nat_zero: #c: curve -> s: scalar_bytes #c ->  Lemma (scalar_as_nat_ s 0 == 0)
+val scalar_as_nat_zero: #c: curve -> s: scalar_bytes #c -> Lemma (scalar_as_nat_ s 0 == 0)
 
 let scalar_as_nat_zero #c s = ()
-
-
 
 
 val scalar_as_nat_def: #c: curve -> s: scalar_bytes #c -> i: nat {i > 0 /\ i <= v (getScalarLen c)} -> Lemma (
